\newpage\section*{Aufgabe 1}
\subsection*{a}
\begin{equation}
\langle N_\text{on}\rangle = s + \alpha \cdot b
\end{equation}
\newpage\section*{Aufgabe 1}
\subsection*{b}
$N_\text{on}$ ist poissonverteilt, $N_\text{off}$ gleichverteilt.
\begin{align}
N_\text{off}&= b\\
N_\text{on} &= \sum_{k=0}^{\infty} \frac{s^k}{k!}\exp(-s) + \alpha \cdot N_\text{off}
\end{align}
\subsection*{c}
Likelihood:
\begin{align}
\mathcal{F}(b,s|x_i) &=  \frac{s^{x_i-\alpha b}}{(x_i-\alpha b)!}\exp(-s)\\
\mathcal{F}(b,s|x_1,...,x_n) &= \prod\limits_{i=1}^{n} \frac{s^{x_i-\alpha b}}{(x_i-\alpha b)!}\exp(-s)
\end{align}
negative Likelihood:
\begin{align}
\mathcal{F}(b,s|x_1,...,x_n) &=  1- \ln \mathcal{L}(b,s|x_1,...,x_n) \\
&= - \sum\limits_{i=1}^{n} \biggl[\ln{s^{x_i-\alpha b}}-\ln{(x_i-\alpha b)!} - s\biggr]\\
&\approx - \sum\limits_{i=1}^{n} \biggl[\ln{s^{x_i-\alpha b}}- (x_i-\alpha b)\cdot(\ln(x_i-\alpha b)-1) - s\biggr]  %Stirling formel?
\end{align}
\subsection*{d}
Minima der negativen Likelihood bestimmen:
\begin{align}
0 &=\frac{\partial\mathcal{F}(b,s)}{\partial s} \\
&= \sum_i \frac{\partial_s\mathcal{L}(b,s|x_i)}{\mathcal{L}(b,s|x_i)}\\
&= \sum_i\biggl((x_i-\alpha b)s^{-1}-1\biggr)\\
n&= \sum_i\biggl((x_i-\alpha b)s^{-1}\biggr)\label{n}\\
ns&= \sum_i\biggl(x_i-\alpha b\biggr)\\
\overline{x}&= \alpha b +s
\end{align}
\begin{align}
0 &=\frac{\partial\mathcal{F}(b,s)}{\partial b} \\
&\approx \sum_i \partial_b \ln s^{x_i-\alpha b} - \partial_b (x_i-\alpha b)\cdot(\ln(x_i-\alpha b)-1)\\
&= \sum_i \partial_b (x_i-\alpha b)\ln s + \alpha (\ln(x_i-\alpha b)-1) - (x_i-\alpha b)\partial_b\ln(x_i-\alpha b))\\
&= \sum_i -\alpha\ln s + \alpha \ln(x_i-\alpha b)\\
0&= n \ln s - \sum_i \ln(x_i-\alpha b)\label{n2}
\end{align}
Einsstzen von n (\ref{n} in \ref{n2}):
\begin{align}
0&= \sum_i\biggl((x_i-\alpha b)s^{-1}\biggr) \ln s - \sum_i \ln(x_i-\alpha b)\\
\ln s\sum_i(x_i-\alpha b)  &= s\sum_i \ln(x_i-\alpha b)
\end{align}
